\documentclass[10pt,a4paper]{article}
\usepackage[latin1]{inputenc}
\usepackage{amsmath}
\usepackage{amsfonts}
\usepackage{amssymb}
\usepackage{graphicx}
\author{Daniel Frederico Lins Leite}
\title{Gaussian Maximum Likelihood}
\newcommand{\distas}[1]{\mathbin{\overset{#1}{\kern\z@\sim}}}%
\newsavebox{\mybox}\newsavebox{\mysim}
\newcommand{\distras}[1]{%
	\savebox{\mybox}{\hbox{\kern3pt$\scriptstyle#1$\kern3pt}}%
	\savebox{\mysim}{\hbox{$\sim$}}%
	\mathbin{\overset{#1}{\kern\z@\resizebox{\wd\mybox}{\ht\mysim}{$\sim$}}}%
}
\begin{document}
	\maketitle
	
	\section{Gaussian Maximum Likelihood}
	\begin{align*}
		X \overset{iid}{\sim} N(\mu,\sigma^2)\\
		L(theta|X) &= p(X|theta)\\
		&= p(X|\mu,\sigma^2)\\
		&= \prod{p(x_i|\mu,\sigma^2)}\\
		\\
		\max_{\mu,sd}{L(theta|X)} &= \max_{\mu,\sigma^2}{\prod{p(x_i|\mu,\sigma^2)}}\\
		&= \max_{\mu,\sigma^2}{ln(\prod{p(x_i|\mu,\sigma^2)))}}\\
		&= \max_{\mu,\sigma^2}{\sum{ln(p(x_i|\mu,\sigma^2))}}\\
		\\
		p(x|\mu,\sigma^2) = \frac{1}{\sqrt{2\pi\sigma^2}} e^{-\frac{(x-\mu)^2}{2\sigma^2}}
		\\
		&= \max_{\mu,\sigma^2}{\sum{ln(\frac{1}{\sqrt{2\pi\sigma^2}} e^{-\frac{(x_i-\mu)^2}{2\sigma^2}})}}\\
		&= \max_{\mu,\sigma^2}{\sum{\big[ln(\frac{1}{\sqrt{2\pi\sigma^2}})+ln( e^{-\frac{(x_i-\mu)^2}{2\sigma^2}})\big]}}\\
		&= \max_{\mu,\sigma^2}{\sum{\big[ln(\frac{1}{\sqrt{2\pi\sigma^2}})+-\frac{(x_i-\mu)^2}{2\sigma^2}\big]}}\\
		&= \max_{\mu,\sigma^2}{\sum{\big[ln(\frac{1}{\sqrt{2\pi\sigma^2}})\big]-\sum{\big[\frac{(x_i-\mu)^2}{2\sigma^2}\big]}}}\\
		&= \max_{\mu,\sigma^2}{\sum{\big[ln((2\pi\sigma^2)^{\frac{1}{2}})\big]-\sum{\big[\frac{(x_i-\mu)^2}{2\sigma^2}\big]}}}\\
		&= \max_{\mu,\sigma^2}{\big[ln((2\pi\sigma^2)^{\frac{1}{2}})\big]\sum{1}-\sum{\big[\frac{(x_i-\mu)^2}{2\sigma^2}\big]}}\\
		&= \max_{\mu,\sigma^2}{\big[\frac{1}{2}ln(2\pi\sigma^2)\big]\sum{1}-\sum{\big[\frac{(x_i-\mu)^2}{2\sigma^2}\big]}}\\
		&= \max_{\mu,\sigma^2}{\big[\frac{1}{2}ln(2\pi\sigma^2)\big]N-\sum{\big[\frac{(x_i-\mu)^2}{2\sigma^2}\big]}}\\
	\end{align*}
	
	TODO
	
	\begin{align*}
		\overset{*}{\mu} &= \frac{1}{N}\sum{x_i}\\
		\overset{*}{\sigma^2}&=\frac{1}{N}\sum{(x_n-\overset{*}{\mu})^2}
	\end{align*}
\end{document}