\documentclass{article}
\usepackage[latin1]{inputenc}
\usepackage{amsmath}
\usepackage{amsfonts}
\usepackage{amssymb}
\usepackage{graphicx}
\usepackage{hyperref}
\usepackage{pgfplots}
\begin{document}
	Exercise 1.4.71\\
	Prove by induction on $n$ that 
	$$ \sum_{i=0}^{n}{i^2} = \frac{n(n+\frac{1}{2})(n+1)}{3}$$
	\\
	Proof by Induction:
	\\
	Base:\\
	\\
	\begin{align*}
		i &= 0\\
		\sum_{i=0}^{0}{i^2} &= 0\\
		\frac{n(n+\frac{1}{2})(n+1)}{3}	&= \frac{0(0+\frac{1}{2})(0+1)}{3}\\
		&= 0\\
	\end{align*}
	\\
	Step:\\
	\\
	\begin{align*}
		\sum_{i=0}^{n+1}{i^2} &= \frac{(n+1)((n+1)+\frac{1}{2})((n+1)+1)}{3}\\
		&=\frac{(n+1)(n+1+\frac{1}{2})(n+1+1)}{3}\\
		&=\frac{(n+1)(n+\frac{3}{2})(n+2)}{3}\\
		&=\frac{(n+1)(n^2+2n+\frac{3}{2}n+\frac{6}{2})}{3}\\
		&=\frac{(n+1)(n^2+2n+\frac{3}{2}n+3)}{3}\\
		&=\frac{(n+1)(n^2+2n+\frac{3}{2}n+3)-3(n+1)^2}{3}+(n+1)^2\\
		&=\frac{(n+1)(n^2+2n+\frac{3}{2}n+3)-3(n+1)(n+1)}{3}+(n+1)^2\\		
		&=\frac{(n+1)[(n^2+2n+\frac{3}{2}n+3)-3(n+1)]}{3}+(n+1)^2\\				
		&=\frac{(n+1)[n^2+2n+\frac{3}{2}n+3-3n-3]}{3}+(n+1)^2\\				
	\end{align*}
	\begin{align*}		
		&=\frac{(n+1)[n^2+\frac{4}{2}n+\frac{3}{2}n+3-\frac{6}{2}n-3]}{3}+(n+1)^2\\								
		&=\frac{(n+1)[n^2+\frac{1}{2}n+3-3]}{3}+(n+1)^2\\				
		&=\frac{(n+1)[n^2+\frac{1}{2}n]}{3}+(n+1)^2\\						
		&=\frac{(n+1)[n(n+\frac{1}{2})]}{3}+(n+1)^2\\		
		&=\frac{(n+1)n(n+\frac{1}{2})}{3}+(n+1)^2\\		
		&=\frac{n(n+\frac{1}{2})(n+1)}{3}+(n+1)^2\\	
		&=\bigg[\sum_{i=0}^{n}{i^2}\bigg]+(n+1)^2\\
		\square					
	\end{align*}
\end{document}