\documentclass{article}
\usepackage[latin1]{inputenc}
\usepackage{amsmath}
\usepackage{amsfonts}
\usepackage{amssymb}
\usepackage{graphicx}
\usepackage{hyperref}
\begin{document}
	Exercise 1.4.44\\
	Let C be any nonsingular matrix. Show that $(C^{-1})^T = (C^T)^{-1}$. 
	\begin{align*}
		C*C^{-1}&=I\\	
		(C*C^{-1})^T&=I^T\\
		C^T*(C^{-1})^T&=I^T\\		
		(C^T)^{-1}C^T*(C^{-1})^T&=(C^T)^{-1}*I^T\\		
		I*(C^{-1})^T&=(C^T)^{-1}*I^T\\	
		I*(C^{-1})^T&=(C^T)^{-1}*I\\
		(C^{-1})^T&=(C^T)^{-1}*I\\		
		(C^{-1})^T&=(C^T)^{-1}\\		
		\square
	\end{align*}
\end{document}