\documentclass{article}
\usepackage[latin1]{inputenc}
\usepackage{amsmath}
\usepackage{amsfonts}
\usepackage{amssymb}
\usepackage{graphicx}
\begin{document}
	Exercise 1.3.23\\
	Prove that if $G$ is triangular, then $det(G) = g_{11}*g_{22}*...*g_{NN}$\\
	\\
	Definition:\\
	\\
	\begin{align*}
		S_{N} = \text{All permutations of 1..N}\\
		\det(A)=\sum _{\sigma \in S_{N}}\left(\operatorname {sgn}(\sigma )\prod _{i=1}^{n}a_{i,\sigma _{i}}\right)
	\end{align*}
	\\
	Case 1: Lower Triangular
	\begin{align*}
	G &= \begin{bmatrix}
	x_{11} & 0      & 0      & \dots  & 0 \\
	x_{21} & x_{22} & 0      & \dots  & 0 \\
	x_{31} & x_{32} & x_{33} & \dots  & 0 \\
	\vdots & \vdots & \vdots & \ddots & \vdots \\
	x_{N1} & x_{N2} & x_{N3} & \dots  & x_{dN}
	\end{bmatrix}\\
	det(G) &= \sum _{\sigma \in S_{N}}\left(\operatorname {sgn}(\sigma )\prod _{i=1}^{n}g_{i,\sigma _{i}}\right)\\	
	\end{align*}
	but 
	\begin{align*}
		A_{ij} &= 0 \text{ if } j > i \text{ (Lower Triangular definition) }\\
		\forall{(\sigma_{i} > i)} &\prod _{i=1}^{n}g_{i,\sigma _{i}} = 0\\
	\end{align*}
	So we can remove these elements of $S_n$ because they will nullify the product.\\
	\begin{align*}	
		\omega &= S_n - \{\sigma | \sigma_i > i\}\\
		&= \{[1...N]\}
	\end{align*}
	so
	\begin{align*}
		det(G) &= \sum _{\sigma \in \omega}\left(\operatorname {sgn}(\sigma )\prod _{i=1}^{n}g_{i,\sigma _{i}}\right)\\
		&= \left(\operatorname {sgn}( [1...N] ) \prod _{i=1}^{n}g_{i,i}\right)\\	
		&= \left(1 * \prod _{i=1}^{n}g_{i,i}\right)\\
		&= g_{11}*g_{22}*...*g_{NN}
	\end{align*}
	
	Case 2: Upper Triangular\\
	Exactly the same as the Lower Triangular.\\

\end{document}